Related.v
@@ -1,0 +1,18 @@
+Require Import Background.
+
+(* Monadic lenses *)
+
+Record mLens (S A : Type) (m : Type -> Type) `{Monad m} := mkMLens
+{ mview : S -> A
+; mupdate : S -> A -> m S
+}.
+Arguments mview [S A m _].
+Arguments mupdate [S A m _].
+Arguments mkMLens [S A m _].
+
+Record mLensLaws {S A m} `{Monad m} (mln : mLens S A m) := mkMLensLaws
+{ mview_mupdate : forall s, mupdate mln s (mview mln s) = ret s
+; mupdate_mview : forall B (k : S -> A -> m B) s a, 
+                    mupdate mln s a >>= (fun s' => k s' (mview mln s')) =
+                    mupdate mln s a >>= (fun s' => k s' a)
+}.
